
## Spicy

> [!abstract] Regn ut.
> 1. $\displaystyle{\frac{3}{2}\left( 7 + \frac{3\  + \ \frac{1}{5}}{\frac{2}{3}} \right) - 1}$
> 2. $\displaystyle{\frac{\left( \frac{4}{7}\  \cdot \ 2\ \frac{3}{5} \right)\  - \ 3}{\frac{2}{3}} + 8}$
> 3. $\displaystyle{\frac{\frac{4}{3}\  + \ 5}{\frac{3}{4}\  + \ \frac{3}{5}} + \frac{7}{2}\left( 1 - \frac{8}{3} \right)}$
> 4. $\displaystyle{\left( \frac{\left( 2\ \ :\ \frac{2}{3} \right)\  \cdot \ \frac{3}{2}}{1\  + \ \frac{3}{2}} - \frac{4}{5} \right) \cdot \left( \frac{4}{5} - 2 \right)}$
> 5. $\displaystyle{\frac{\frac{-3}{4}+\frac{1}{3}}{\frac{1}{6}}+ 2\left( \frac{5}{3}-\frac{2}{6} \right)}$
> 6. $\displaystyle{\left(\frac{\left(\frac{1}{7}-\frac{1}{2}\right)}{\left(\frac{1}{2}+\frac{3}{7}\right)}\right)+ 2\left( \frac{1}{2}-\frac{8}{26} \right)}$
> 7. $\displaystyle{\left(\frac{\left( 2:\frac{1}{6} \right)\cdot 5}{2-\frac{4}{3}}- 10\right)\cdot \left( \frac{5}{8}-\frac{1}{2} \right)}$

> [!note]- LÃ¸sning 
> 1. 
> $$
> \begin{align*}\frac{3}{2}\left( 7 + \frac{16}{5} \cdot \frac{3}{2} \right) - 1& = \frac{3}{2} \cdot \frac{35 + 24}{5} - 1\\& = \frac{177}{10} - \frac{10}{10}\\& = \frac{167}{10}\end{align*}
> $$
> 2. 
> $$
> \begin{align*}\frac{4 \cdot 13-105}{7 \cdot 5} \cdot \frac{3}{2} + 8&= {\frac{53}{7 \cdot 5} \cdot \frac{3}{2} + 8}\\&= {\frac{-159\cdot 3}{7\cdot 5\cdot 2} + \frac{560}{7\cdot 5\cdot 2}}\\& = \frac{401}{70}\end{align*}
> $$
> 3. 
> $$
> \begin{align*}\frac{19}{3} \cdot \frac{20}{27} + \frac{7}{2} \cdot \left( - \frac{5}{3} \right) & =\frac{380}{81} - \frac{35}{6}\\&= \frac{760}{162} - \frac{945}{162}\\& = - \frac{185}{162}\end{align*}
> $$
>  4.
>  $$
>  \begin{align*}{\left( \left( 2 \cdot \frac{3}{2} \cdot \frac{3}{2} \right) \cdot \frac{2}{5} - \frac{4}{5} \right) \cdot \left( - \frac{6}{5} \right)}&= {\left( \frac{9}{5} - \frac{4}{5} \right) \cdot \left( - \frac{6}{5} \right)}\\& = {- \frac{6}{5}}\end{align*}
>  $$
> 5.
> $$
> \begin{align*}\frac{\frac{-3}{4}+\frac{1}{3}}{\frac{1}{6}}+ 2(\frac{5}{3}-\frac{2}{6}) & = \frac{\frac{-9+4}{12}}{\frac{1}{6}}+2(\frac{10-2}{6})\\& =\frac{\frac{-5}{12}\cdot \frac{6}{1}}{\frac{1}{6}\frac{6}{1}}+2\cdot \frac{8}{6}\\& = \frac{-5}{2}+\frac{16}{6} = \frac{-15+16}{6} = \frac{1}{6}\end{align*}
> $$
> 6. 
> $$
> \begin{align*}\left(\frac{\left(\frac{1}{7}-\frac{1}{2}\right)}{\left(\frac{1}{2}+\frac{3}{7}\right)}\right)+ 2(\frac{1}{2}-\frac{8}{26}) & =\frac{\frac{2-7}{14}}{\frac{7+6}{14}} +2(\frac{13-8}{26})\\& =\frac{\frac{-5}{14}\cdot 14}{\frac{13}{14}\cdot 14} + \frac{5}{13}\\& = \frac{-5}{13}+\frac{5}{13} = 0\end{align*}
> $$
> 7.
> $$
> \begin{align*}\left(\frac{(2:\frac{1}{6})\cdot 5}{2-\frac{4}{3}}- 10\right)\cdot (\frac{5}{8}-\frac{1}{2})& =\left(\frac{12\cdot 5}{\frac{6-4}{3}} - 10 \right)\cdot(\frac{5-4}{8})\\& = \left(\frac{12\cdot 5\cdot 3}{\frac{2}{3}\cdot 3} - 10\right)\cdot \frac{1}{8}\\& =\left(\frac{180}{2}- 10 \right)\cdot \frac{1}{8} = 80\cdot \frac{1}{8} = 10\end{align*}
> $$

